Arithmetic/theories/Languages/MiniC/Semantics.v
@@ -1,0 +1,253 @@
+From RAC Require Import Utils Environnement.
+From RAC.Languages Require Import Syntax.
+From Coq Require Import Strings.String ZArith.ZArith.
+From RecordUpdate Require Import RecordUpdate.
+Import RecordSetNotations.
+
+Declare Scope c_sem_scope.
+Delimit Scope c_sem_scope with csem.
+
+Declare Scope generic_stmt_sem_scope.
+Delimit Scope generic_stmt_sem_scope with gssem.
+
+Declare Scope generic_exp_sem_scope.
+Delimit Scope generic_exp_sem_scope with gesem.
+
+
+Definition compiler_prefix : id := "_".
+Definition comp_var x : id  := (compiler_prefix ++ x)%string.
+Definition is_comp_var := String.prefix compiler_prefix.
+Definition res_f : id := comp_var "res".
+
+Definition exp_sem_sig {T : Set} : Type := Env -> @_c_exp T -> 𝕍 -> Prop.
+Definition stmt_sem_sig {S T: Set} : Type  :=  @fenv S T -> Env -> @_c_statement S T ->  Env -> Prop.
+Definition Empty_exp_sem {T: Set} : @exp_sem_sig T := fun _ _ _ => False.
+Definition Empty_stmt_sem {S T: Set} : @stmt_sem_sig S T := fun _ _ _ _ => False.
+
+
+
+(* extensible expression semantic *)
+Inductive generic_exp_sem {T:Set} {ext_exp : @exp_sem_sig T} (ev:Env): @_c_exp T -> 𝕍 -> Prop :=
+| C_E_Int (z:Z) irz : ev |= z => VInt (z ⁱⁿᵗ irz)
+| C_E_Var (x:𝓥) z : 
+    ev x = Some (Def (VInt z)) -> 
+    ev |=  (C_Id x C_Int) => z
+| C_E_BinOpInt e e' (z z':Z) op z_ir z'_ir
+    (H:Int.inRange (⋄ op z z')) :
+    ev |= e =>  VInt (z ⁱⁿᵗ z_ir) ->
+    ev |= e' =>  VInt (z' ⁱⁿᵗ z'_ir) ->
+    ev |=  BinOpInt e op e' => VInt ((⋄ op) z z' ⁱⁿᵗ H)
+| C_E_BinOpTrue e e' (z z' : Z) z_ir z'_ir op :
+    ev |= e => VInt (z ⁱⁿᵗ z_ir) ->
+    ev |= e' => VInt (z' ⁱⁿᵗ z'_ir) ->
+    (◁ op) z z' = true ->
+    ev |= BinOpBool e op e' => VInt one
+| C_E_BinOpFalse e e' (z z' : Z) op z_ir z'_ir :
+    ev |= e => VInt (z ⁱⁿᵗ z_ir) -> 
+    ev |= e' => VInt (z' ⁱⁿᵗ z'_ir) -> 
+    ((◁ op) z z' = false ) ->
+    ev |= BinOpBool e op e' => VInt zero
+(* | C_Ext x v t: 
+    (* variable must not be of type int (treated by C_E_Var) *)
+    t <> C_Int ->
+    
+    (* variable must be bound and init *)
+    ev x = Some (Def v) ->
+
+
+    (* the external semantic can only add additional constraint, the result is always v *)
+    ext_exp ev (C_Id x t) v ->
+
+    ev |= (C_Id x t) => v *)
+
+where  "env '|=' e => z" := (generic_exp_sem env e z) : generic_exp_sem_scope.
+#[global] Hint Constructors generic_exp_sem  : rac_hint.
+
+Definition c_exp_sem := @generic_exp_sem Empty_set Empty_exp_sem.
+Notation "Ω '|=' e => v"  := (c_exp_sem Ω e v) : c_sem_scope.
+
+Open Scope utils_scope.
+Open Scope mini_c_scope.
+
+(* extensible statement semantic *)
+Inductive generic_stmt_sem {S T: Set} {ext_exp: @exp_sem_sig T} {ext_stmt: @stmt_sem_sig S T} (f : @fenv S T) (ev:Env) : @_c_statement S T -> Env -> Prop := 
+    | S_skip  :  (ev |= <{ skip }> => ev) f
+    | S_Assign x z (e : @_c_exp T) : 
+        (* must not be a compiler variable i.e. function return value *)
+        is_comp_var x = false ->
+
+        type_of_value (ev x) = Some C_Int ->
+        (* value returned must be of same type*)
+        type_of_value (Some z) = Some C_Int ->
+
+        @generic_exp_sem T ext_exp ev e z -> 
+        (ev |= <{x = e}> => (ev <| env ; vars ::= {{x\z}} |>)) f
+
+    | S_IfTrue ev' z e s s' :
+        @generic_exp_sem T ext_exp ev e z /\ ~ (z = VInt zero) ->
+        (ev  |= s => ev') f ->
+        (ev  |= <{ if e s else s'}> => ev') f
+
+    | S_IfFalse ev' e s s' :
+        @generic_exp_sem T ext_exp ev e (VInt zero) ->
+        (ev |= s' => ev') f ->
+        (ev |= <{ if e s else s'}> => ev') f
+
+    | S_While e s  ev' :
+        (ev |= <{ if e s ; while e s else skip }> => ev') f ->
+        (ev |= <{ while e s }> => ev') f
+
+    | S_Seq  ev' ev'' s s' :
+        (ev |= s => ev') f ->
+        (ev' |= s' => ev'') f ->
+        (ev |= <{ s ; s' }> =>  ev'') f
+
+    | S_FCall fname (b: @_c_statement S T) ev' c xargs eargs (zargs : 𝕍 ⃰ ) z : 
+        List.length xargs = List.length eargs ->
+        f.(funs) fname = Some (xargs,b) ->
+        List.Forall2 (@generic_exp_sem T ext_exp ev) eargs zargs ->
+        (empty_env <| env ; vars ::= p_map_addall_back xargs zargs |> |= b => ev') f -> 
+        ~ List.In res_f (stmt_vars b) -> 
+        ev' res_f = Some (Def z) -> (* must be a defined value *)
+        (ev |= (FCall c fname eargs) => ev <| env ; vars ::= {{c\Def z}} |> <| mstate := ev' |>) f
+
+    | S_PCall p b ev' xargs eargs zargs : 
+        List.length xargs = List.length eargs ->
+        f.(procs) p = Some (xargs,b) ->
+        List.Forall2 (@generic_exp_sem T ext_exp ev) eargs zargs ->
+        (empty_env <| env ; vars ::= p_map_addall_back xargs zargs |> |= b => ev') f -> 
+        (ev |= PCall p eargs => ev <| mstate := ev' |>) f
+
+    | S_Return e z : 
+        (* not allowed to return an unassigned value *)
+        @generic_exp_sem T ext_exp ev e (Def z) ->
+        (ev |= <{ return e }> => ev <| env ; vars ::= {{res_f\Def z}} |>) f
+
+    | S_PAssert  e z :
+        @generic_exp_sem T ext_exp ev e z -> z <> VInt zero ->
+        (ev |= <{ assert e }> => ev) f
+
+    | S_ExtSem s ev' :  
+        (* only S_Ext constructor allowed to use external semantic*)
+        ext_stmt f ev (S_Ext s) ev' 
+        -> (ev |= (S_Ext s) => ev') f
+    
+    where "env |= s => env'"  := (fun f => generic_stmt_sem f env s env') : generic_stmt_sem_scope.
+    
+#[global] Hint Constructors generic_stmt_sem  : rac_hint.
+
+
+(* 
+Declare Scope c_sem_scope.
+Delimit Scope c_sem_scope with csem. 
+Definition c_stmt_sem := @generic_stmt_sem Empty_set Empty_set Empty_exp_sem Empty_stmt_sem.
+Notation "ev |= s => ev'"  := (c_stmt_sem ev s ev') : c_sem_scope. 
+*)
+
+
+
+(* 
+Definition c_decl_sem (env env':Ω) (mem mem':𝓜) d : Prop := 
+forall x t u,
+env x  = None -> 
+(ty u) = Some t ->
+d = C_Decl t x -> env' = env <| vars ::= {{x\u}} |> /\ mem = mem'.
+*)
+
+
+Definition _untouched_var_same_eval_exp {T : Set} (exp_sem : @exp_sem_sig T) := 
+    forall (ev:Env) (e: @_c_exp T) v x,
+    ~ List.In v (exp_vars e) -> 
+    exp_sem ev e x ->
+    (forall x', exp_sem (ev <| env ; vars ::= {{v\x'}} |>)  e x)
+    /\ 
+    (forall l z', 
+    _no_env_mpz_aliasing ev ->
+    ev v = Some (Def (VMpz (Some l))) -> exp_sem (ev <| mstate ::= {{l\z'}} |>) e x).
+
+
+
+Definition _untouched_var_same_eval_stmt {S T : Set} (exp_sem : @exp_sem_sig T) (stmt_sem : @stmt_sem_sig S T) := 
+    forall f ev ev' (s: @_c_statement S T) x, 
+    stmt_sem f ev s ev' ->
+    ~ List.In x (stmt_vars s) /\ is_comp_var x = false -> 
+    ev x = ev' x
+.
+
+Definition _no_mem_aliasing {S T : Set} (stmt_sem : @stmt_sem_sig S T)  : Prop := 
+    forall (exp_sem:@exp_sem_sig T) f (ev:Env) s (ev':Env), 
+    _no_env_mpz_aliasing ev
+    -> stmt_sem f ev s ev' 
+    -> _no_env_mpz_aliasing ev'.
+
+
+Definition _determinist_exp_eval {T : Set} (exp_sem : @exp_sem_sig T) : Prop := 
+forall e ev v,  exp_sem ev e v ->  (forall v', exp_sem ev e v' -> v = v')
+.
+
+
+Definition _determinist_stmt_eval {S T : Set} (ext_exp_sem : @exp_sem_sig T) (stmt_sem : @stmt_sem_sig S T) : Prop := 
+    @_determinist_exp_eval T ext_exp_sem  -> 
+    forall f s ev ev',  stmt_sem f ev s ev' ->  (forall ev'', stmt_sem f ev s ev'' -> ev' = ev'').
+
+Definition _weakening_of_expression_semantics {T} (exp_sem : @exp_sem_sig T) : Prop := 
+    forall e ev (x:𝕍), 
+    exp_sem ev e x <-> (forall ev',  (ev ⊑ ev')%envmem -> exp_sem ev' e x).
+
+
+Definition _weakening_of_statement_semantics_1  {S T : Set} (exp_sem : @exp_sem_sig T) (stmt_sem : @stmt_sem_sig S T) := 
+    (*
+    should be in both directions according to the article but right to left does not work :
+    We will see if the 'bad' direction is used in the proof 
+    If this is the cast, one direction is trying to add to have a new env_01 = ev_0 + a and a new env_02 = ev_0 + b so that 
+        (ev0 + a) inter ev0 + b) = ev1
+    *)  
+    _weakening_of_expression_semantics exp_sem ->
+    forall (f : @fenv S T) ev₀ s ev₁,
+    stmt_sem f ev₀ s ev₁ ->
+    ( forall ev₀', (ev₀  ⊑ ev₀')%envmem ->
+    exists ev₁' , (ev₁  ⊑ ev₁')%envmem /\ stmt_sem f ev₀' s ev₁').
+
+
+Definition _weakening_of_statement_semantics_2  {S T : Set} (exp_sem : @exp_sem_sig T) (stmt_sem : @stmt_sem_sig S T) := 
+    
+    forall (f: @fenv S T) ev₀ ev₀' s ev₁,
+    _determinist_exp_eval exp_sem ->
+    _weakening_of_expression_semantics exp_sem ->
+    stmt_sem f ev₀ s ev₁ /\ (ev₀ ⊑ ev₀')%envmem  ->
+    (
+        forall ev₁',
+        stmt_sem f ev₀' s ev₁'->
+        (* if v is a compiler variable, i.e. a function return value, v can change*)
+        (forall (v:𝓥), (v ∉ ev₀) /\ is_comp_var v = false  -> ev₀' v = ev₁' v) 
+        /\
+        (forall (x:location) (v:𝓥), ev₀ v <> Some (Def (VMpz x)) -> ev₀'.(mstate) x = ev₁'.(mstate) x)
+    ).
+
+
+Definition _weakening_of_expression_semantics_3 {T : Set} (exp_sem : @exp_sem_sig T) := 
+    forall ev e z ev₀,
+    exp_sem ev e z ->
+    forall ev₀', (ev₀' ⊑ ev₀)%envmem ->
+    (
+        (forall v, (dom ev₀ - dom ev₀') v /\ ~ List.In v (exp_vars e))
+        /\
+        (forall x v, (dom ev₀.(mstate) - dom ev₀'.(mstate)) x ->  ev₀ v = Some (Def (VMpz x)) /\ ~ List.In v (exp_vars e))
+    ) ->
+
+    exp_sem  ev₀' e z
+.
+
+Definition _weakening_of_statement_semantics_3  {S T : Set} (stmt_sem : @stmt_sem_sig S T) := 
+    forall f ev₀  s ev₁,
+    stmt_sem f ev₀ s ev₁ -> 
+    (
+        forall ev₀', (ev₀' ⊑ ev₀)%envmem ->
+        (
+            (forall v, (dom ev₀ - dom ev₀') v /\ ~ List.In v (stmt_vars s))
+            /\
+            (forall x v, (dom ev₀.(mstate) - dom ev₀'.(mstate)) x -> ev₀ v = Some (Def (VMpz x)) /\ ~ List.In v (stmt_vars s))
+        ) ->
+
+        exists ev₁', stmt_sem f ev₀' s ev₁'
+    ).
