Arithmetic/theories/Languages/MiniFSL/Semantics.v
@@ -1,0 +1,102 @@
+From RAC Require Import Utils Environnement.
+From RAC.Languages Require Import Syntax MiniC.Semantics.
+From Coq Require Import Strings.String ZArith.ZArith BinaryString.
+From RecordUpdate Require Import RecordUpdate.
+Import RecordSetNotations.
+
+Open Scope utils_scope.
+Open Scope mini_c_scope.
+
+Inductive fsl_term_sem (f: @fenv _fsl_statement Empty_set) (ev:Env) : ℨ -> Z -> Prop :=
+    | S_T_Int z : fsl_term_sem f ev (T_Z z) z 
+    
+    | S_T_LVar x z : ev.(binds) x = Some z -> fsl_term_sem f ev (T_Id x FSL_Integer) z
+
+    | S_T_Var x v : ev.(env) v = Some (Def (VInt x)) ->  fsl_term_sem f ev (T_Id v FSL_Int) x ̇ 
+
+    | S_T_BinOpInt t t' z zint z' z'int op :  
+        fsl_term_sem f ev t z ->
+        fsl_term_sem f ev t' z' ->
+        ~ (op = FSL_Div /\ z = 0)%type ->
+        fsl_term_sem f ev (T_BinOp t op t') ((fsl_binop_int_model op) zint z'int)
+
+    | S_T_CondTrue p t z t':
+        fsl_pred_sem f ev p BTrue ->
+        fsl_term_sem f ev t z ->
+        fsl_term_sem f ev (T_Cond p t t') z
+
+    |S_T_CondFalse p t t' z':
+        fsl_pred_sem f ev p BFalse ->
+        fsl_term_sem f ev t' z' ->
+        fsl_term_sem f ev (T_Cond p t t') z'
+
+    | S_T_Call fname b xargs targs zargs z :
+        List.length xargs = List.length targs ->
+        f.(lfuns) fname = Some (xargs,b) ->
+        List.Forall2 (fsl_term_sem f ev) targs zargs ->
+        fsl_term_sem f (empty_env <| env ; binds ::= p_map_addall_back xargs zargs |>) b z -> 
+        fsl_term_sem f ev (T_Call fname targs) z 
+
+
+with fsl_pred_sem (f: @fenv _fsl_statement Empty_set) (ev:Env) :  𝔅 -> 𝔹 -> Prop :=
+    | S_P_True : fsl_pred_sem f ev P_True BTrue
+    | S_P_False : fsl_pred_sem f ev P_False BFalse
+
+    | S_P_BinOpTrue t t' z z' (op:fsl_binop_bool): 
+        fsl_term_sem f ev t z ->
+        fsl_term_sem f ev t' z' ->
+        (fsl_binop_bool_model op) z z' ->
+        fsl_pred_sem f ev (P_BinOp t op t) BTrue
+
+    | S_P_BinOpFalse t t' z z' (op:fsl_binop_bool): 
+        fsl_term_sem f ev t z ->
+        fsl_term_sem f ev t' z' ->
+        ~ (fsl_binop_bool_model op) z z' ->
+        fsl_pred_sem f ev (P_BinOp t op t) BFalse
+
+    | S_P_NotTrue p : 
+        fsl_pred_sem f ev p BTrue ->
+        fsl_pred_sem f ev (P_Not p) BFalse
+
+    | S_P_NotFalse p : 
+        fsl_pred_sem f ev p BFalse ->
+        fsl_pred_sem f ev (P_Not p) BTrue 
+
+    | S_P_DisjLeftTrue p p' : 
+        fsl_pred_sem f ev p BTrue ->
+        fsl_pred_sem f ev (P_Disj p p') BTrue 
+
+    | S_P_DisjLeftFalse p p' z : 
+        fsl_pred_sem f ev p BFalse ->
+        fsl_pred_sem f ev p' z ->
+        fsl_pred_sem f ev (P_Disj p p') z
+    
+    | S_P_Call p b xargs targs zargs z :
+        List.length xargs = List.length targs ->
+        f.(preds) p = Some (xargs,b) ->
+        List.Forall2 (fsl_term_sem f ev) targs zargs ->
+        fsl_pred_sem f (empty_env <| env ; binds ::= p_map_addall_back xargs zargs |>) b z -> 
+        fsl_pred_sem f ev (P_Call p targs) z 
+.
+
+#[global] Hint Constructors fsl_term_sem : rac_hint.
+#[global] Hint Constructors fsl_pred_sem : rac_hint.
+
+Declare Scope fsl_sem_scope.
+Delimit Scope fsl_sem_scope with fslsem.
+
+(* Notation "Ω '|=' t => v" := (fsl_term_sem Ω t v) : fsl_sem_scope. *)
+
+Inductive _fsl_assert_sem  (f : fenv ) (ev:Env) : fsl_statement -> Env -> Prop :=
+| FSL_Assert (p:𝔅) : 
+    fsl_pred_sem f ev p BTrue ->
+    _fsl_assert_sem f ev (LAssert p) ev
+.
+
+#[global] Hint Constructors _fsl_assert_sem : rac_hint.
+
+
+Definition fsl_stmt_sem := @generic_stmt_sem _fsl_statement Empty_set Empty_exp_sem _fsl_assert_sem.
+Notation "ev |= s => ev'"  := (fun f => fsl_stmt_sem f ev s ev') : fsl_sem_scope. 
+
+
