Arithmetic/theories/Languages/MiniFSL/Syntax.v
@@ -1,0 +1,88 @@
+From Coq Require Import ZArith.ZArith String.
+From RAC Require Import Notations.
+From RAC.Languages Require Import MiniC.Syntax MiniGMP.Syntax.
+
+
+Inductive fsl_type := FSL_Int (* machine integer *) | FSL_Integer. (* mathematical integer *)
+
+Inductive fsl_binop_bool :=  FSL_Lt | FSL_Le | FSL_Gt | FSL_Ge | FSL_Eq | FSL_NEq.
+Definition fsl_binop_bool_model (x:fsl_binop_bool) : Z -> Z -> Prop := match x with
+    | FSL_Lt => Z.lt
+    | FSL_Le => Z.le
+    | FSL_Gt => Z.gt
+    | FSL_Ge => Z.ge
+    | FSL_Eq => Z.eq
+    | FSL_NEq => fun x y => ~(Z.eq x y)
+end.
+
+Inductive fsl_binop_int := FSL_Add | FSL_Sub  | FSL_Mul  | FSL_Div.
+Definition fsl_binop_int_model (x:fsl_binop_int) : Z -> Z -> Z := match x with
+    | FSL_Add => Z.add
+    | FSL_Sub => Z.sub
+    | FSL_Mul => Z.mul
+    | FSL_Div => Z.div
+end.
+
+
+Inductive fsl_decl : Set :=  FSL_Decl (τ:gmp_t) (name:id). (* logic declaration δ *)
+
+Inductive predicate : Set :=
+    | P_True | P_False (* truth values *)
+    | P_BinOp (lt: fsl_term) (op:fsl_binop_bool) (rt : fsl_term)
+    | P_Not (t:predicate)
+    | P_Disj (lp:predicate) (rp:predicate)  (* disjunction *)
+    | P_Call (name:string) (args:fsl_term ⃰) (* predicate call *)
+with fsl_term :=
+    | T_Z (z:Z) :> fsl_term (* integer in Z *)
+    | T_Id (name:id) (ty:fsl_type)  (* variable access, ty added to distinguish between program var and logic var *)
+    | T_BinOp (lt : fsl_term) (op:fsl_binop_int) (rt : fsl_term)
+    | T_Cond (cond:predicate) (_then:fsl_term) (_else:fsl_term) (* conditional term *)
+    | T_Call (name:string) (args:fsl_term ⃰) (* logic function call *)
+.
+
+Notation 𝔅 := predicate. (* predicates *)
+Notation ℨ := fsl_term. (* logical terms *)
+
+
+
+Inductive _fsl_statement : Set := LAssert (p:predicate). (* logic assertion *)
+
+
+Coercion fsl_binop_int_to_c (x:fsl_binop_int) : c_binop_int := match x with
+    | FSL_Add => C_Add
+    | FSL_Sub => C_Sub
+    | FSL_Mul => C_Mul
+    | FSL_Div => C_Div
+end.
+Notation "□" := fsl_binop_int_to_c.
+
+Coercion fsl_binop_bool_to_c (x:fsl_binop_bool) : c_binop_bool := match x with
+    | FSL_Lt => C_Lt
+    | FSL_Le => C_Le 
+    | FSL_Gt => C_Gt
+    | FSL_Ge => C_Ge
+    | FSL_Eq => C_Eq 
+    | FSL_NEq => C_NEq
+end.
+Notation "◖" := fsl_binop_bool_to_c.
+
+Inductive _fsl_routine : Set :=
+| LFun (ret:fsl_type) (name:id) (args: fsl_decl ⃰) (body:fsl_term) (* logic function *)
+| Predicate (name:id) (args: fsl_decl ⃰) (p:predicate) (* predicate *)
+.
+
+Definition fsl_routine := @_c_routine _fsl_routine _fsl_statement Empty_set.
+
+
+Definition op (x:fsl_binop_int) : id -> id -> id -> _gmp_statement := match x with
+| FSL_Add => GMP_Add
+| FSL_Sub => GMP_Sub
+| FSL_Mul => GMP_Mul
+| FSL_Div => GMP_Div
+end.
+
+(***** Printing *****)
+
+Notation "'/*@' 'logic' k id '(' x ',' .. ',' y ')' '=' t '*/'" := (F_Ext (LFun k id (cons x .. (cons y nil) ..) t)) (in custom c_decl at level 0): mini_c_scope.
+Notation "'/*@' 'predicate' id '(' x ',' .. ',' y ')' '=' p '*/'" := (F_Ext (Predicate id (cons x .. (cons y nil) ..) p)) (p custom c_stmt, in custom c_decl at level 0): mini_c_scope.
+Notation "'/*@' 'assert' p '*/'" := (S_Ext (LAssert p)) (in custom c_stmt at level 0) : mini_c_scope.
