Arithmetic/theories/Languages/MiniGMP/Lemmas.v
@@ -1,0 +1,69 @@
+From RAC Require Import Utils Environnement.
+From RAC.Languages Require Import Syntax Semantics MiniC.Lemmas. 
+From RecordUpdate Require Import RecordUpdate.
+From Coq Require Import ZArith.ZArith.
+Open Scope Z_scope. 
+
+Lemma _weakening_of_gmp_statements_semantics_1 : 
+    _weakening_of_statement_semantics_1 Empty_exp_sem _gmp_stmt_sem
+.
+Proof with eauto using eq_env_partial_order, eq_mem_partial_order,refl_env_mem_partial_order with rac_hint ; try easy.
+    intros Hweak f ev₀ s ev₁.
+    - intro Hderiv. induction Hderiv; intros ev₀' [Henv Hmem]; epose proof (fun y => weakening_of_c_expression_semantics y ev₀) as weak_exp.
+        (* init *)
+        * exists (ev₀' <| env ; vars ::= {{x \ Def (VMpz (Some l))}} |> <| mstate ::= {{l \Defined 0}} |> ). split.
+            + split. 
+                ++ apply env_partial_order_add... 
+                ++ apply mems_partial_order_add...
+            + apply S_init.
+                ++ intros v Hcontra. 
+                    (* the fact v is not bound to mpz location l by Ω₀ doesn't mean 
+                        that v will also not be bound to mpz location l by Ω₀' 
+                    *) 
+                    admit.
+                ++ (* the semantic of ⊑ only ensures a defined mpz must stay the same, 
+                        but here, x points to an undefined mpz value so it can be either stay like so or
+                        be defined 
+                    *)
+                    admit.
+        (* clear *)
+        * exists (ev₀' <| env ; vars ::= {{x\Def (VMpz None)}} |><| mstate ::= {{a \ Undefined u}} |>). split.
+            + split.
+                ++ apply env_partial_order_add...
+                ++ apply mems_partial_order_add...
+            + constructor... 
+
+        (* set_i *)
+        * exists (ev₀' <| mstate ::= {{a \ Defined (z) ̇}} |>). split.
+            + split... intro n. apply (mems_partial_order_add ev₀ ev₀' Hmem a z ̇).  
+            + apply S_set_i. eapply eq_env_partial_order... apply weak_exp...   
+
+        (* set_z *)
+        * exists (ev₀' <| mstate ::= {{a \ z}} |>). split.
+            + split... intro n0.  apply (mems_partial_order_add ev₀ ev₀' Hmem a).
+            + apply S_set_z with n...
+
+        (* get_int *)
+        *  eexists (ev₀' <| env ; vars ::= fun e =>  e{x \ Def (VInt (zy ⁱⁿᵗ ir))} |>)...  split.
+            + split... simpl. pose proof env_partial_order_add...
+            + apply S_get_int with ly...
+        
+        (* set_s *)
+        * exists (ev₀' <| mstate ::= {{lx \ Defined zx}} |>). split.
+            + split... apply (mems_partial_order_add ev₀ ev₀' Hmem lx zx). 
+            + constructor...
+
+        (* cmp *)
+        *  eexists (ev₀' <| env ; vars ::= fun e => e{c \ b} |>). split.
+            + split... simpl. pose env_partial_order_add...
+            + apply S_cmp with lx ly zx zy...        
+        
+        (* op *)
+        * eexists (ev₀' <| mstate ::= {{lr \Defined (⋄ bop zx zy)}} |>). split.
+            + split... intro n. apply mems_partial_order_add...   
+            + apply S_op with lx ly ; try apply weak_exp...  
+Admitted.
+
+Definition weakening_of_gmp_statements_semantics_1 := 
+    weakening_of_statement_semantics_1 Empty_exp_sem _gmp_stmt_sem _weakening_of_gmp_statements_semantics_1.
+
