Arithmetic/theories/Languages/MiniGMP/Semantics.v
@@ -1,0 +1,115 @@
+From RAC Require Import Utils Environnement.
+From RAC.Languages Require Import Syntax.
+From RAC.Languages Require Import MiniC.Semantics MiniGMP.Syntax.
+From Coq Require Import Strings.String ZArith.ZArith BinaryString.
+From RecordUpdate Require Import RecordUpdate.
+Import RecordSetNotations.
+
+Open Scope utils_scope.
+Open Scope mini_c_scope.
+Open Scope mini_gmp_scope.
+Declare Scope gmp_stmt_sem_scope.
+Delimit Scope gmp_stmt_sem_scope with gmpssem.
+
+
+(* Definition undef_type (u:undef) := match u with UMpz _ => Mpz | UInt _ => C_Int end. *)
+
+Inductive _gmp_stmt_sem { S T : Set } (f : @fenv S T) (ev:Env) : gmp_statement -> Env -> Prop := 
+    | S_init x (l:location):
+        (forall v, ev v <> Some (Def (VMpz (Some l)))) ->
+        (exists n, ev x = Some (Undef (UMpz n)))%type ->
+        (ev |= <(init(x))> => ev <| env ; vars ::= {{x\Def (VMpz (Some l))}} |> <| mstate ::= {{l\Defined 0}} |>) f
+    
+    | S_clear x a u:   
+        ev x = Some (Def (VMpz (Some a))) ->   
+        (ev |= <(cl(x))> => ev <| env ; vars ::= {{x\(Def (VMpz None))}} |> <| mstate ::= {{a\Undefined u}} |>) f
+
+    | S_set_i x y z a :  
+        ev x = Some (Def (VMpz (Some a))) ->
+        (ev |= y => VInt z)%csem ->
+        (ev |= <(set_i(x,y))> => ev <| mstate ::= {{a\Defined (z ̇)}} |>) f
+
+    | S_set_z x y z (a n : location) :  
+        ev x = Some (Def (VMpz a)) ->
+        ev y = Some (Def (VMpz n)) ->
+        ev.(mstate) n = Some z ->
+        (ev |= <(set_z(x,y))> => ev <| mstate ::= {{a\z}} |>) f 
+
+    | S_get_int x y ly zy (ir:Int.inRange zy) :
+        ev y = Some (Def (VMpz (Some ly))) ->
+        ev.(mstate) ly = Some (Defined zy) -> 
+        (ev |= <(x = get_int(y))> => ev <| env ; vars ::= {{x\VInt (zy ⁱⁿᵗ ir) : 𝕍}} |>) f
+
+    | S_set_s s x zx lx :
+        ev x = Some (Def (VMpz (Some lx))) ->
+        BinaryString.to_Z s = zx ->
+        (ev |= <(set_s(x,s))> => ev <| mstate ::= {{lx\Defined zx}} |> ) f
+
+    | S_cmp c x (lx ly :location) zx y zy (b:𝕍):
+        ev x = Some (Def (VMpz (Some lx))) ->
+        ev y = Some (Def (VMpz (Some ly))) ->
+        ev.(mstate) lx = Some (Defined zx) ->
+        ev.(mstate) ly = Some (Defined zy) ->
+        (
+            (Z.gt zx zy <-> b = VInt one) /\
+            (Z.lt zx zy <-> b = VInt sub_one) /\
+            (Z.eq zx zy <-> b = VInt zero)
+        ) ->
+        (ev |= <(c = cmp(x,y))> => ev <| env ; vars ::= {{c\b}} |>) f
+    
+    | S_op bop r lr x y (lx ly : location) zx zy :
+        ev x = Some (Def (VMpz (Some lx))) ->
+        ev y = Some (Def (VMpz (Some ly))) ->
+        ev.(mstate) lx = Some (Defined zx) ->
+        ev.(mstate) ly = Some (Defined zy) ->
+        ev r = Some (Def (VMpz (Some lr))) -> (* not in paper *)
+        (ev |= op bop r x y => ev <| mstate ::= {{lr\Defined (⋄ (□ bop) zx zy) }} |>) f
+
+where "ev |= s => ev'" := (fun f => _gmp_stmt_sem f ev s ev') : gmp_stmt_sem_scope.
+
+#[global] Hint Constructors _gmp_stmt_sem  : rac_hint.
+
+
+
+
+Definition gmp_stmt_sem := @generic_stmt_sem _gmp_statement _gmp_t Empty_exp_sem _gmp_stmt_sem.
+(*
+Notation "Ω ⋅ M |= s => Ω' ⋅ M'"  := (fun f => gmp_stmt_sem f Ω M s Ω' M') : gmp_sem_scope. 
+ *)
+
+
+ Fact _no_mem_aliasing_gmp : _no_mem_aliasing _gmp_stmt_sem.
+Proof with auto with rac_hint.
+    intros exp_sem f ev s ev' Hnoalias H. induction H
+    ; auto ;  try (rename v into l1) ;
+    intros v v' ll l' Hvv' Hl Hl' leq ; subst ; autounfold with rac_hint in * ; simpl in *.
+    - destruct (eq_dec x v).
+        + subst. autounfold with rac_hint in *. rewrite p_map_same in Hl. rewrite p_map_not_same in Hl'... inversion Hl. 
+            subst. now destruct H with v'.
+        + rewrite p_map_not_same in Hl... destruct (eq_dec x v').
+            * subst. rewrite p_map_same in Hl'. inversion Hl'. subst. now destruct H with v.
+            * rewrite p_map_not_same in Hl'... destruct Hnoalias with v v' l' l'...
+    - destruct (eq_dec x v).
+        + subst. now rewrite p_map_same in Hl.
+        + rewrite p_map_not_same in Hl... destruct (eq_dec l' a).
+            * destruct Hnoalias with v x l' a... 
+            * destruct (eq_dec x v').
+                ** subst. rewrite p_map_same in Hl'... easy.
+                ** rewrite p_map_not_same in Hl'... destruct Hnoalias with v v' l' l'...     
+    - destruct (string_dec x v').
+        + subst. rewrite p_map_same in Hl'. discriminate.
+        + rewrite p_map_not_same in Hl'... destruct (string_dec x v).
+            * subst. rewrite p_map_same in Hl... discriminate.
+            * rewrite p_map_not_same in Hl... destruct Hnoalias with v v' l' l'...
+    - assert (type_of_value (Some b) = Some C_Int). {
+        destruct H3 as [sup [inf eq]]. destruct (Z.lt_trichotomy zx zy) as [Hinf | [Heq | Hsup]].
+        - apply inf in Hinf. now subst.
+        - apply eq in Heq. now subst.
+        - apply Z.lt_gt in Hsup.  apply sup in Hsup. now subst. 
+        } 
+        destruct (string_dec c v').
+        + subst. rewrite p_map_same in Hl'. injection Hl' as Hl'. now subst. 
+        + rewrite p_map_not_same in Hl'... destruct (string_dec c v).
+            * subst. rewrite p_map_same in Hl. injection Hl as Hl. now subst.
+            * rewrite p_map_not_same in Hl... destruct Hnoalias with v v' l' l'...
+Qed.
