Arithmetic/theories/Notations.v
@@ -1,7 +1,5 @@
-From Coq Require Import ZArith.ZArith.
-From Coq Require Import ZArith.Znat.
-From Coq Require Import Lists.List. 
-From Coq Require Import Strings.String.
+From Coq.ZArith Require Import ZArith Znat.
+From Coq Require Import Lists.List  Strings.String.
 
 
 Declare Scope utils_scope.
@@ -12,8 +10,11 @@ Declare Custom Entry pmap.
 Reserved Notation "X ⇀ Y"  (at level 100).
 Notation "A ⃰" := (list A) (at level 20) : type_scope.
 Notation "x '\' y" := (x,y) (in custom pmap at level 0, x constr, y constr) : utils_scope.
+
 Notation id := string.
 
+Definition 𝓥 : Type := id. (* program variables and routines *)
+Definition 𝔏 : Type := id. (* logic variables *)
 Reserved Notation "⊥".
 Reserved Notation "'dom' f" (at level 10).
 Reserved Notation "f { xy , .. , xy' }" (xy custom pmap, xy' custom pmap, at level 0).
