Arithmetic/theories/Wip.v
@@ -1,0 +1,131 @@
+From RAC Require Import Utils Environnement.
+From RAC.Languages Require Import Syntax.
+From Coq Require Import ZArith.ZArith Strings.String.
+From RecordUpdate Require Import RecordUpdate.
+
+Open Scope utils.
+
+(* invariants for routine translation *)
+
+(* notations *)
+Inductive add_var (e : Env) (τ:gmp_t) (v:id) (z:Z) : Env -> Prop :=
+| typeInt irz : 
+    τ = C_Int ->
+    add_var e τ v z (e <| env ; vars ::= {{v\(VInt (z ⁱⁿᵗ irz)) :𝕍}} |>)%utils
+
+| typeMpz x (n:Int.MI) :
+    τ  = Mpz ->
+    (forall v',  e v' <> Some (Def (VMpz (Some x))) )->
+    add_var e τ v z 
+    ( e 
+    <| env ; vars ::= {{ v\Def (VMpz (Some x)) }} |>
+    <| mstate ::= {{x\Defined (proj1_sig n)}} |> 
+    )
+.
+
+Example add_var_int : forall (ir3 :Int.inRange 3),
+add_var empty_env C_Int "y" 3 (empty_env  <| env ; vars := ⊥{"y"\Def (VInt ( 3ⁱⁿᵗ ir3))} |>).
+Proof. now constructor. Qed.
+
+Definition 𝐴 := list (gmp_t * id * Z).
+
+(* Fixpoint add_var_𝐴 (env : Ω) (mem_state : 𝓜) (A : 𝐴) : Ω * 𝓜 -> Prop := match A with 
+    | nil => fun x => x
+    | cons (t,v,z) tl => fun x => add_var env mem_state t v z (fst x, snd x)
+end. *)
+
+
+(*fixme fixpoint or List.fold *)
+(*)
+Definition add_var_𝐴 (env : Ω) (mem_state : 𝓜) (A : 𝐴) : Prop :=
+    List.fold_left (
+        fun (acc:Prop) (args:gmp_t * id * Z)  => 
+            let '(t,id,z) := args in
+            add_var env mem_state t id z  (env,mem_state) /\ acc 
+    ) A (env,mem_state)
+ . *)
+
+Inductive add_var_𝐴 (e : Env) : 𝐴 -> Env -> Prop := 
+| add_var_nil : add_var_𝐴  e nil e
+
+| add_var_cons t v z A e': 
+    True -> 
+    add_var e t v z e' -> 
+    add_var_𝐴 e A e'
+.
+
+
+
+Example add_var_mpz  : 
+add_var empty_env Mpz "y" 3  
+    ( empty_env 
+        <| env ; vars := ⊥{"y"\Def 1%nat} |>
+        <| mstate := ⊥{(1%nat)\(Defined 3)} |>
+    )
+.
+Proof.
+    assert (ir3: Int.inRange 3). easy.
+    now apply (typeMpz empty_env Mpz "y" 3 1%nat (3ⁱⁿᵗ ir3)).
+Qed.
+
+
+
+(* Compute add_var_𝐴 (⊥,⊥) ⊥ nil. *)
+
+Example envaddnil : add_var_𝐴 empty_env nil empty_env.
+Proof.
+ constructor.
+Qed.
+
+Open Scope list.
+
+Example envaddone : add_var_𝐴 empty_env  ((T_Ext Mpz, "y", 3)::nil) 
+    (empty_env 
+        <| env ; vars := ⊥{"y"\Def (VMpz 1%nat)} |>
+        <| mstate := ⊥{1%nat\(Defined 3)} |>
+    )
+.
+Proof.
+    assert (ir3: Int.inRange 3). easy.
+    eapply add_var_cons with (t:=Mpz) (v:="y") (z:=3).
+ - auto.
+ - apply (typeMpz empty_env Mpz "y" 3 1%nat (3ⁱⁿᵗ ir3)).
+    * reflexivity.
+    * intro v. intro contra. inversion contra.
+Qed.
+
+
+
+
+
+(* synchronicity invariant *)
+Definition I1 (env:Ω) (ienv:Γ) := ((dom env.(binds)) = (dom (fst ienv) + dom (snd ienv)))%utils.
+
+(* suitability invariant *)
+Definition I2 (env:ψ) := True. (* todo *)
+
+
+Inductive pgrm_var_representation (iop:ϴ) (e : Env) (ienv:Γ) : Env -> Prop :=
+| empty ΩΓ 𝓜Γ :   
+    I1 e ienv ->
+    let A := nil  (* { (iop ((snd ienv) v), v, (snd env) v ) | v in dom ienv  } *)
+    in
+    add_var_𝐴 e A {|env:=ΩΓ; mstate:=𝓜Γ|} -> 
+    pgrm_var_representation iop e ienv{|env:=ΩΓ; mstate:=𝓜Γ|}
+.
+
+(* Definition well_formed_program :=
+    - all variables declared before usage
+    - all functions defined before called
+    - well typed
+*)
+
+
+
+(* Module Todo.
+Hypothesis type_soundness : forall (env:Ω) (t:Z), True.
+
+Hypothesis convergence : forall (type_env:Γ) (r:mini_c(((((((((_routines), 
+    exists (t:T), type_env r = t.
+End Todo. *)
+
